@prefix rdf: <http://www.w3.org/1999/02/22-rdf-syntax-ns#> .
@prefix imf: <http://ns.imfid.org/imf#> .
@prefix pav: <http://purl.org/pav/> .
@prefix o-rdf: <http://tpl.ottr.xyz/rdf/0.1/> .
@prefix o-owl-rstr: <http://tpl.ottr.xyz/owl/restriction/0.1/> .
@prefix owl: <http://www.w3.org/2002/07/owl#> .
@prefix xsd: <http://www.w3.org/2001/XMLSchema#> .
@prefix skos: <http://www.w3.org/2004/02/skos/core#> .
@prefix rdfs: <http://www.w3.org/2000/01/rdf-schema#> .
@prefix ex: <http://example.com#> .
@prefix sh: <http://www.w3.org/ns/shacl#> .
@prefix o-imf: <http://ns.imfid.org/templates/> .
@prefix ottr: <http://ns.ottr.xyz/0.4/> .
@prefix o-owl-ma: <http://tpl.ottr.xyz/owl/macro/0.1/> .
@prefix o-owl-ax: <http://tpl.ottr.xyz/owl/axiom/0.1/> .
@prefix shsh: <http://www.w3.org/ns/shacl-shacl#> .

imf:Aspect
    a owl:Class ;
    skos:example "Function, Location, Product are examples of aspects." ;
    skos:prefLabel "Aspect" ;
    skos:scopeNote """

  viewpoint
  modalitity

  """ .

imf:AspectObject
    a owl:Class ;
    rdfs:subClassOf [
        a owl:Restriction ;
        owl:onClass imf:Aspect ;
        owl:onProperty imf:hasAspect ;
        owl:qualifiedCardinality "1"^^xsd:nonNegativeInteger
    ] ;
    skos:definition """

    An aspect object describes an asset from a specific viewpoint (or
    aspect).

    An aspect object has a single aspect, we say that the aspect
    object \"is of\" this aspect.

    """ ;
    skos:prefLabel "Aspect Object" .

imf:MultiAspectObject
    a owl:Class ;
    skos:prefLabel "Multi-Aspect Object" ;
    skos:scopeNote """

  A multi-aspect object is a collection of aspect objects that
  describe an asset from different viewpoints (aspects). 

  There are currently no formal restrictions on the aspect objects
  that a multi-aspect object groups together. Hence, a multi-aspect
  object may collect aspect objects of the same aspect, or of
  different aspects.

  """ .

imf:associativeRelation
    a owl:ObjectProperty ;
    rdfs:domain imf:AspectObject ;
    rdfs:range imf:AspectObject ;
    rdfs:subPropertyOf skos:related ;
    owl:propertyDisjointWith imf:hierachicalRelation ;
    skos:definition "A generic associative relation." ;
    skos:prefLabel "associative relation" ;
    skos:scopeNote """
    
      This relation is used to enforce that subproperties respect this
      relation's definition. This must be enforced by introducing
      class axioms that locally further restrict the domain and range
      of the relation.
      
    """ .

imf:hasAspect
    a owl:ObjectProperty ;
    rdfs:domain imf:AspectObject ;
    rdfs:range imf:Aspect ;
    skos:definition "Relates an aspect object to its aspect." ;
    skos:prefLabel "has aspect" .

imf:hasAspectObject
    a owl:ObjectProperty ;
    rdfs:domain imf:MultiAspectObject ;
    rdfs:range imf:AspectObject ;
    skos:definition """

    Relates the multi-aspect object to the aspect object(s) it
    collects.

    """ ;
    skos:prefLabel "has aspect object" .

imf:hierarchicalRelation
    a owl:IrreflexiveProperty, owl:ObjectProperty ;
    rdfs:domain imf:AspectObject ;
    rdfs:range imf:AspectObject ;
    rdfs:subPropertyOf skos:semanticRelation ;
    skos:definition "A generic hierachical relation that may be used to represent a breakdown structure." ;
    skos:prefLabel "hierarchical relation" ;
    skos:scopeNote """
    
      This relation is used to enforce that subproperties respect this
      relation's definition. This must be enforced by introducing
      class axioms that locally further restrict the domain and range
      of the relation.
      
    """ .

imf:intraAspectRelation
    a owl:ObjectProperty ;
    rdfs:domain imf:AspectObject ;
    rdfs:range imf:AspectObject ;
    rdfs:subPropertyOf skos:semanticRelation ;
    skos:definition "A generic relation between aspect objects of the same aspect" ;
    skos:prefLabel "intra-aspect relation" ;
    skos:scopeNote """
    
      This relation is used to enforce that subproperties respect this
      relation's definition. This must be enforced by introducing
      class axioms that locally further restrict the domain and range
      of the relation.
      
    """ .

<http://ns.imfid.org/imf-top>
    a owl:Ontology ;
    owl:imports <http://www.w3.org/2004/02/skos/core> ;
    owl:versionIRI <http://ns.imfid.org/ontology/20220701/imf-top> ;
    skos:altLabel "IMF top ontology" ;
    skos:prefLabel "Information Modelling Framework Ontology: Top Ontology " ;
    skos:scopeNote """

      This ontology defines the very core classes and relations of the
      Information Modelling Framework (IMF) to provide a structure for
      ontologies that extend this ontology.

    """ .

[]
    a owl:AllDisjointClasses ;
    owl:members (imf:Aspect
        imf:AspectObject
        imf:MultiAspectObject
    ) .

