@prefix xsd:	<http://www.w3.org/2001/XMLSchema#> .
@prefix rdf:	<http://www.w3.org/1999/02/22-rdf-syntax-ns#> .
@prefix rdfs:	<http://www.w3.org/2000/01/rdf-schema#> .
@prefix owl:    <http://www.w3.org/2002/07/owl#> .
@prefix skos:	<http://www.w3.org/2004/02/skos/core#> .
@prefix pav:	<http://purl.org/pav/> .
@prefix sh: 	<http://www.w3.org/ns/shacl#> . 
@prefix shsh:   <http://www.w3.org/ns/shacl-shacl#> .
@prefix ex:	<http://example.com#> .
@prefix imf:	<http://ns.imfid.org/imf#> .

@prefix p14:    <http://example.com/P14#> .
@prefix ottr:        <http://ns.ottr.xyz/0.4/> .
@prefix o-rdf:       <http://tpl.ottr.xyz/rdf/0.1/> .
@prefix o-rdfs:       <http://tpl.ottr.xyz/rdfs/0.2/> .
@prefix o-owl-ax:    <http://tpl.ottr.xyz/owl/axiom/0.1/> .
@prefix o-owl-ma:    <http://tpl.ottr.xyz/owl/macro/0.1/> .
@prefix o-owl-rstr:  <http://tpl.ottr.xyz/owl/restriction/0.1/> .

@prefix o-imf:	     <http://ns.imfid.org/templates/> .
@prefix o-imf-t-s:   <http://ns.imfid.org/templates/type/shacl/> .


<http://ns.imfid.org/imf> a owl:Ontology ;
    owl:versionIRI <http://ns.imfid.org/20230331/imf> ;
    owl:imports
      <http://ns.imfid.org/20230331/imf-elements> ,
      <http://ns.imfid.org/20230331/imf-aspects> ,
      <http://ns.imfid.org/20230331/imf-attributes>
      #<http://ns.imfid.org/20230331/imf-types> 
    ;
    skos:prefLabel "Information Modelling Framework Ontology " ;
    skos:altLabel "IMF ontology" ;
    skos:scopeNote """

      This is the main IMF ontology and its main point of entry.  This
      ontology document imports all other IMF sub-ontology documents, each
      of which focus on one particular part of the ontology.

    """;

    .

imf:externalReference a owl:ObjectProperty ;
    skos:definition "A generic relation that is used to relate elements to external ontologies or reference data library for added semantic descriptions." .

imf:hierarchicalRelation a owl:ObjectProperty ;
    # a owl:IrreflexiveProperty ; ### An error occurred during reasoning: Non-simple property '<http://ns.imfid.org/imf#hierarchicalRelation>' or its inverse appears in irreflexive object property axiom..
    skos:prefLabel "hierarchical relation";
    rdfs:subPropertyOf skos:semanticRelation ;
    rdfs:domain imf:AspectElement ;
    rdfs:range imf:AspectElement ;
    skos:definition "A generic hierachical relation that may be used to represent a breakdown structure." ;
    
    .

imf:associativeRelation a owl:ObjectProperty ;
    skos:prefLabel "associative relation";
    rdfs:subPropertyOf skos:related ;
    owl:propertyDisjointWith imf:hierachicalRelation ;
    rdfs:domain imf:AspectElement ;
    rdfs:range imf:AspectElement ;
    skos:definition "A generic associative relation." ;
    
    .
